---
layout: post
section-type: post
title: Math Techniques for Quantum Mechanics\\量子力学的数学工具
category: diary
tags: [ 'tutorial' ]
---
<script type="text/javascript"
    src="http://cdn.mathjax.org/mathjax/latest/MathJax.js?config=TeX-AMS-MML_HTMLorMML">
</script>

>等等
>这是chem356**quantum chemistry**中的Chapter2学习总结

Math Techniques for Quantum Mechanics\\量子力学的数学工具
======================================================
1. Intro to differential equations\\微分式子基础
------------------------------------------------------

### second-order homogeneous linear differential equation with constant coefficients\\二阶常系数齐次线性方程

$$\lambda^2-2\lambda-3=0$$

It's simple to solve the equation in three steps//很简单分三步：


	1. find the eigen equation\\求特征方程；
	2. calculate the eigen value\\算特征根；
	3. get the get the general solutions\\得到对应齐次方程通解

>eg:
找到\\(\frac{d^2y}{dx^2}-2\frac{dy}{dx}-3y=0\\)的通解
eigen equation\\特征方程:
$\lambda^2-2\lambda-3=0$
eigen value\\特征根：
$\lambda_1 = 3, \lambda_2 = -1$
general solutions\\通解：
$Y = C_1 e^{3x} + C_2 e^{-x}$

### second order non homogeneous linear differential equation with constant coefficient\\二阶常系数非齐次线性方程

对于$\frac{d^2y}{dx^2}＋a\frac{dy}{dx}+by=f(x)$，首先要找到对应的齐次方程$\frac{d^2y}{dx^2}＋a\frac{dy}{dx}+by=0$的通解$Y$，再找到原非齐次方程的一个特解 $y^\*$，则原非齐次方程的通解 $y=Y+y^*$

Case1: $f(x)=Ax + B$
>eg:
找到$\frac{d^2y}{dx^2}-2\frac{dy}{dx}-3y=3x+1$的通解

>设特解$y^* = Ax + B$

>代入原方程得：$-2A - 3(Ax + B) = 3x + 1$

>解得: $A=-1, B=1/3$

>解出特解: $y^*=-x+1/3$

>所以通解为: $y= C_1 e^{3x} + C_2 e^{-x} -x + 1/3$

Case2: $f(x)=Q(x) e^{rx}$
>eg:
找到$\frac{d^2y}{dx^2}-3\frac{dy}{dx}+2y=xe^{2x}$的通解

>eg:
找到$\frac{d^2y}{dx^2}-6\frac{dy}{dx}+9y=xe^{3x}$的通解

case3: $f(x) = e^{rx} (Acos\omega x + Bsin\omega x )$

>eg:
找到$\frac{d^2y}{dx^2}+2\frac{dy}{dx}+2y=10sin2x$的通解

>eg:
找到$\frac{d^2y}{dx^2}+4y=10sin2x$的通解

2. Partial differential equations and separation of variables\\偏微分方程和分离变量法
------------------------------------------------------

3. Intro to Statistics\\统计基础
------------------------------------------------------

$variance = \sigma^2 = E[\frac{1}{n-1} \sum^n_{i=1} (x_i-\bar{x})^2] = E[\frac1n \sum^n_{i=1} (x_i-\mu)^2]$

前一项无偏，而若写成$\frac{1}{n} \sum^n_{i=1} (x_i-\bar{x})^2$则会低估方差

